Test.lean
@@ -3,5 +3,6 @@ module
 public import Test.Deps
 public import Test.Collect
 public import Test.Extract
+public import Test.Spec
 
 @[expose] public section
